[broken] tranform

Primitive_Matchers/Transform.thy
@@ -6,6 +6,81 @@ imports "Common_Primitive_Matcher"
         "../Primitive_Matchers/IpAddresses_Normalize"
 begin
 
+(*closure bounds*)
+
+(*def: transform_optimize = optimize_matches opt_MatchAny_match_expr \<circ> optimize_matches optimize_primitive_univ
+apply before and after nralizatin and closures
+*)
+
+(*this cannot be normalized as it can contain MatchNot MatchAny*)
+definition transform_optimize_strict :: "common_primitive rule list \<Rightarrow> common_primitive rule list" where 
+    "transform_optimize_strict = optimize_matches (opt_MatchAny_match_expr \<circ> optimize_primitive_univ)"
+
+theorem transform_optimize_strict: assumes simplers: "simple_ruleset rs" and wf\<alpha>: "wf_unknown_match_tac \<alpha>"
+      shows "(common_matcher, \<alpha>),p\<turnstile> \<langle>transform_optimize_strict rs, s\<rangle> \<Rightarrow>\<^sub>\<alpha> t \<longleftrightarrow> (common_matcher, \<alpha>),p\<turnstile> \<langle>rs, s\<rangle> \<Rightarrow>\<^sub>\<alpha> t"
+      and "simple_ruleset (transform_optimize_strict rs)"
+      and "\<forall> m \<in> get_match ` set rs. \<not> has_disc C m \<Longrightarrow> \<forall> m \<in> get_match ` set (transform_optimize_strict rs). \<not> has_disc C m"
+      and "\<forall> m \<in> get_match ` set rs. normalized_nnf_match m \<Longrightarrow> \<forall> m \<in> get_match ` set (transform_optimize_strict rs). normalized_nnf_match m"
+      and "\<forall> m \<in> get_match ` set rs. normalized_n_primitive disc_sel f m \<Longrightarrow> \<forall> m \<in> get_match ` set (transform_optimize_strict rs). normalized_n_primitive disc_sel f m"
+  proof -
+    let ?\<gamma>="(common_matcher, \<alpha>)"
+    let ?fw="\<lambda>rs. approximating_bigstep_fun ?\<gamma> p rs s"
+
+    show simplers_transform: "simple_ruleset (transform_optimize_strict rs)"
+      unfolding transform_optimize_strict_def
+      using simplers optimize_matches_simple_ruleset by fast
+
+    have 1: "?\<gamma>,p\<turnstile> \<langle>rs, s\<rangle> \<Rightarrow>\<^sub>\<alpha> t \<longleftrightarrow> ?fw rs = t"
+      using approximating_semantics_iff_fun_good_ruleset[OF simple_imp_good_ruleset[OF simplers]] by fast
+    have rs: "?fw rs = ?fw (transform_optimize_strict rs)"
+      unfolding transform_optimize_strict_def
+      apply(rule optimize_matches[symmetric])
+      using optimize_primitive_univ_correct_matchexpr opt_MatchAny_match_expr_correct by (metis comp_apply)
+    have 2: "?fw (transform_optimize_strict rs) = t \<longleftrightarrow> ?\<gamma>,p\<turnstile> \<langle>transform_optimize_strict rs, s\<rangle> \<Rightarrow>\<^sub>\<alpha> t "
+      using approximating_semantics_iff_fun_good_ruleset[OF simple_imp_good_ruleset[OF simplers_transform], symmetric] by fast
+    from 1 2 rs show "?\<gamma>,p\<turnstile> \<langle>transform_optimize_strict rs, s\<rangle> \<Rightarrow>\<^sub>\<alpha> t \<longleftrightarrow> ?\<gamma>,p\<turnstile> \<langle>rs, s\<rangle> \<Rightarrow>\<^sub>\<alpha> t" by simp
+
+    { fix P m
+      assume p1: "\<forall>m. P m \<longrightarrow> P (optimize_primitive_univ m)"
+      assume p2: "\<forall>m. P m \<longrightarrow> P (opt_MatchAny_match_expr m)"
+      from p1 p2 have "\<forall> m \<in> get_match ` set rs. P m \<Longrightarrow> \<forall> m \<in> get_match ` set (transform_optimize_strict rs). P m"
+        unfolding transform_optimize_strict_def optimize_matches_def
+        by(induction rs) (simp_all)
+    } note matchpred_rule=this
+
+    { fix m
+      have "\<not> has_disc C m \<Longrightarrow> \<not> has_disc C (optimize_primitive_univ m)"
+      by(induction m rule: optimize_primitive_univ.induct) simp_all
+    } moreover { fix m 
+      have "\<not> has_disc C m \<Longrightarrow> \<not> has_disc C (opt_MatchAny_match_expr m)"
+      by(induction m rule: opt_MatchAny_match_expr.induct) simp_all
+    } ultimately show "\<forall> m \<in> get_match ` set rs. \<not> has_disc C m \<Longrightarrow> \<forall> m \<in> get_match ` set (transform_optimize_strict rs). \<not> has_disc C m"
+      using matchpred_rule[of "\<lambda>m. \<not> has_disc C m"] by fast
+    
+    { fix m
+      {fix a
+       have "optimize_primitive_univ (Match a) = Match a \<or> optimize_primitive_univ (Match a) = MatchAny"
+        by(induction "(Match a)" rule: optimize_primitive_univ.induct) auto
+      } note matcha_cases=this
+      have "normalized_nnf_match m \<Longrightarrow> normalized_nnf_match (optimize_primitive_univ m)"
+      apply(induction m rule: optimize_primitive_univ.induct)
+      apply simp_all
+      apply(case_tac m)
+          apply(simp_all)
+      apply(case_tac "optimize_primitive_univ (Match a) = Match a")
+       apply(simp)
+      apply(case_tac "optimize_primitive_univ (Match a) = MatchAny")
+       apply(simp)
+      
+      
+    } moreover { fix m 
+      have "\<not> has_disc C m \<Longrightarrow> \<not> has_disc C (opt_MatchAny_match_expr m)"
+    } ultimately show "\<forall> m \<in> get_match ` set rs. \<not> has_disc C m \<Longrightarrow> \<forall> m \<in> get_match ` set (transform_optimize_strict rs). \<not> has_disc C m"
+      using matchpred_rule[of "\<lambda>m. \<not> has_disc C m"] by fast
+  
+  qed
+
+
 definition transform_strict :: "common_primitive rule list \<Rightarrow> common_primitive rule list" where 
     "transform_strict = optimize_matches opt_MatchAny_match_expr(*^^10)*) \<circ> normalize_rules_dnf \<circ> optimize_matches optimize_primitive_univ \<circ> rw_Reject \<circ> rm_LogEmpty"
 
